%!Mode:: "TeX:UTF-8"
%!TEX TS-program = xelatex
\documentclass{ctexart}
\newif\ifpreface
%\prefacetrue
\input{../../../global/all}
\begin{document}
\large
\iffalse
  \setlength{\baselineskip}{1.2em}
  \ifpreface
    \input{../../../global/preface}
  \else
    \maketitle
  \fi
\fi
\newgeometry{left=2cm,right=2cm,top=2cm,bottom=2cm}
%from_here_to_type
\begin{problem}\label{pro:1}
  Assume \((N(t):t \geq 0)\) is a renewing process with renewing internal
  \(\{\xi_n: n \geq 1\}\), \(S_n=\sum_{k=1}^{n} \xi_k\), \(N(t):=\sup \{n: S_n \leq t\}\), calculate \(g(t):=\mathbb{E}(N(t)^2)\).
\end{problem}
\begin{solution}
  Let \(T_1=\xi_1\), then \(g(t)=\mathbb{E}(\mathbb{E}(N(t)^2 \mid T_1))=\int_{0}^t \mathbb{E}(N(t)^2 \mid T_1=x)d F(x)\).
  By the independence, \[
    \mathbb{E}(N(t)^2 \mid T_1=x)=\begin{cases}
      0                          & , x > t    \\
      \mathbb{E}((1 + N(t-x))^2) & , x \leq t
    \end{cases}
  \]
  That is \(\mathbb{E}(N(t)^2 \mid T_1=x)=\begin{cases}
    0                    & ,x > t    \\
    1 + 2m(t-x) + g(t-x) & ,x \leq t
  \end{cases}\).
  Therefore,
  \[
    g(t)=F(t) + 2\int_{0}^t m(t-x)d F(x) + \int_{0}^t g(t-x)d F(x)
  \]
  So \(g(t)=2m(t)-F(t) + \int_{0}^t g(t-x)d F(x)\).
  Thus, \(g(t)=2m(t)-F(t) + (2m-F)*m(t)\), so \(g(t)=m(t) + 2m * m(t)\).
\end{solution}

\begin{problem}\label{pro:2}
  Assume renewing internal time obey \(U(0,1)\). \(0 < t< 1\), calculate the distrubution of \(S_{N(t)}\)
  and \(\mathbb{E}(S_{N(t)})\).
\end{problem}
\begin{solution}
  By calculating, \(m(t)=\mathrm{e}^t-1, 0 < t< 1\). \(\forall 0 \leq s \leq t <1\), \[
    \mathbb{P}(S_{N(t)}\leq s)=1-t + \int_{0}^s(1-t + x)\mathrm{e}^x dx=1-(t-s)\mathrm{e}^s
  \]
  Therefore, \[
    \mathbb{E}(S_{N(t)})=\int_{0}^t s(1-t + s)\mathrm{e}^s ds=\mathrm{e}^t -t -1
  \]
\end{solution}

\begin{problem}\label{pro:3}
  Assume renewing internal time obey random variable \(X\) with distrubution function \(F\).
  Let \(\gamma_t=S_{N(t) + 1}-t\) be the rest lifetime at time \(t\).
  Prove: \[
    \mathbb{P}(\gamma_t > z)=1-F(t + z) + \int_{0}^t(1-F(t + z -x))d m(x)
  \]
\end{problem}
\begin{solution}
  Let \(A_z(t)=\mathbb{P}(\gamma_t > z)\), then \[
    \mathbb{P}(\gamma_t > z \mid \xi_1=x)=\begin{cases}
      1        & ,x > t + z         \\
      0        & , t < x \leq t + z \\
      A_z(t-x) & , 0 < x \leq t
    \end{cases}
  \]
  Then,
  \[
    A_z(t)=\int_{0}^\infty \mathbb{P}(\gamma_t > z \mid \xi_1=x)d F(x)=1-F(t + z) + \int_{0}^tA_z(t-z)dF(x)
  \]
  Thus, \[
    A_z(t)=1-F(t + z) + \int_{0}^\infty(1-F(t + z -x))dm(x)
  \]
\end{solution}

\begin{problem}\label{pro:4}
  One kind of devices are replaced as they are worn out.
  Let the lifetime of the devices be sequences
  \(\{\xi_n:n \geq 1\}\), and let \(S_n=\sum_{k=1}^{n} \xi_k\), \(N(t)=\sup \{n: S_n \leq t\}\). \(L(t)=S_{N(t) + 1}-S_{N(t)}\).
  Prove: \(\mathbb{P}(L(t)> x) \geq \mathbb{P}(\xi_1 > x)\).
\end{problem}
\begin{solution}
  When \(t \leq x\), easy to get that \(\mathbb{P}(L(t)>x)=\mathbb{P}(\xi_1>x)\).
  Now we assume \(t > x\).
  \begin{equation}
    \begin{aligned}
      \mathbb{P}(L(t)>x)= & \sum_{k=0}^{\infty} \mathbb{P}\left(\xi_{k+1}>x, N(t)=k\right)                                                           \\
      =                   & \sum_{k=0}^{\infty} \mathbb{P}\left(\xi_{k+1}>x, S_k \leq t, \xi_{k+1}>t-S_k\right)                                      \\
      =                   & \sum_{k=1}^{\infty} \mathbb{P}\left(\xi_{k+1}>x, t-x<S_k \leq t\right)                                                   \\
                          & \quad+\sum_{k=0}^{\infty} \mathbb{P}\left(\xi_{k+1}>t-S_k, S_k \leq t-x\right)                                           \\
      =                   & \mathbb{P}\left(\xi_1>x\right) \mathbb{E}[(N(t)-N(t-x))]+\mathbb{P}(N(t)=N(t-x))                                         \\
      =                   & \mathbb{P}\left(\xi_1>x\right)+\mathbb{P}\left(\xi_1>x\right) \mathbb{E}[(N(t)-N(t-x))-1]                                \\
                          & +\mathbb{P}(N(t)=N(t-x))                                                                                                 \\
      =                   & \mathbb{P}\left(\xi_1>x\right)+\mathbb{P}\left(\xi_1>x\right) \mathbb{E}\left[(N(t)-N(t-x)-1) 1_{\{N(t)>N(t-x)\}}\right] \\
                          & -\mathbb{P}\left(\xi_1>x\right) \mathbb{E}\left(1_{\{N(t)=N(t-x)\}}\right)+\mathbb{P}(N(t)=N(t-x))                       \\
      \geq                & \mathbb{P}\left(\xi_1>x\right) .
    \end{aligned}
  \end{equation}
\end{solution}

\begin{problem}\label{pro:-1}
  Toss a coin until we get two successively head, call it a renew.
  We toss the coin \(k\) times, call the number of renews \(N(k)\).
  Find the distribution and expectation of interval time \(T\)
\end{problem}

\begin{solution}
  Let \(p_n:=\mathbb{P}(T=n)\). Then \(p_1=0,p_2=\frac{1}{4}\).
  Easy to find that \(p_{n+2}=\frac{1}{2}p_{n + 1}+\frac{1}{4}p_{n}\).
  The characteristic equation of this sequence is \(x^2=\frac{1}{2}x+\frac{1}{4}\).
  The roots are \(x_1=\frac{1+\sqrt{5}}{4},x_2=\frac{1-\sqrt{5}}{4}\).
  So \(p_n=Ax_1^n+Bx_2^n\). By \(p_1,p_2\), easy to get that
  \(p_n=\frac{1}{2 \sqrt{ 5}}\left(x_1^{n-1}-x_2^{n-1}\right)\).
  So easily \(\mathbb{E}(T)=\sum_{n=1}^{\infty} np_n=6\).
\end{solution}

\end{document}
