% arara: xelatex
%!Mode:: "TeX:UTF-8"
%!TEX encoding = UTF-8 Unicode
%!TEX TS-program = xelatex
%!language = zh
\documentclass{ctexart}
\newif\ifpreface
\prefacetrue
\input{../../../global/all}
\begin{document}
\large
\setlength{\baselineskip}{1.2em}
\ifpreface
\input{../../../global/preface}
\newgeometry{left=2cm,right=2cm,top=2cm,bottom=2cm}
\else
\newgeometry{left=2cm,right=2cm,top=2cm,bottom=2cm}
\maketitle
\fi
%from_here_to_type
\begin{problem}
  Assume \(V \subset \mathbbm{A}_k^{n}\) is irreducible, and \(p \in V\).
  Let \(m_p := \{f \in k[V] : f(p) = 0\}, M_p := \{f \in k[x_1,\cdots,x_n]: f(p) = 0\}\).
  Prove that \(m_p \cong M_p/\ide(V)\).
\end{problem}

\begin{solution}
  Consider \( \theta : M_p \to m_p ,\theta(f) := f + \ide(V)\).
  Since \( p \in V\) we get \(\theta\) is well-defined.
  And easily we get \(\theta\) is homomorphism. Now consider \(\ker \theta\).
  Obviously \(\ide(V) \subset \ker \theta\), now we prove \(\ker \theta \subset \ide(V)\).
  Assume \( f \in \ker\theta\), to prove \(f \in \ide(V)\).
  Since \(\theta(f)=\ide(V)\), we get \(f+\ide(V)=\ide(V)\), so \(f \in \ide(V)\).
  So \(\ker \theta = \ide(V)\). And easily \(\theta\) is surjective, so we get
  \(m_p=M_p/\ker \theta=M_p / \ide(V)\).
\end{solution}

\begin{problem}
  Prove that \(M_p/M_p^2+\ide(V) \cong m_p/m_p^2\).
\end{problem}
\begin{solution}
  Consider \(\theta : M_p \to m_p/m_p^2, f \mapsto f|_V+m_p^2\). Easily \(\theta\) is homomorphism and surjective.
  Now we prove \(\ker \theta = M_p^2+\ide(V)\).

  On one hand, assume \(f \in \ker \theta\), i.e., \(f|_V \in m_p^2\).
  Then \(\exists g_1,\cdots,g_n,h_1,\cdots,h_n \in m_p\) such that \(f|_V=\sum_{k=1}^{n} g_k h_k\).
  Assume \(g_k=G_k|_V,h_k=H_k|_V\). Then \(G_k,H_k \in M_p\).
  Consider \(f-\sum_{k=1}^{n} G_k H_k=:h \in k[x_1,\cdots,x_n]\), easily to know \(h(x)=0,\forall x \in V\).
  So \(h \in \ide(V)\), thus \(f \in M_p^2+\ide(V)\).

  On the other hand, assume \(f \in M_p^2+\ide(V)\), to prove \(\theta f =0\).
  Assume \(f=\sum_{k=1}^{n} G_k H_k+h\), where \(G_k,H_k \in M_p\) and \(h \in \ide(V)\).
  Then \(\theta f = \sum_{k=1}^{n} g_k h_k +m_p^2\), where \(g_k=G_k|_V,h_k=H_k|_V\).
  So we get \(\theta f = m_p^2=0\).

  Finally we get \(m_p/m_p^{2} = M_p/ \ker \theta = M_p / M_p^2+\ide(V)\).
\end{solution}
\begin{problem}\label{pro:1}
  Assume \(V \subset \mathbbm{A}_k^n\) is irreducible, and \(p \in V,f \in k[V], f(p)\neq 0\).
  Consider \(V_f:= \{x \in V: f(x)\neq 0 \}\). Let \(\theta: V_f \to \mathbbm{A}_k^{n+1},x \mapsto (x,\frac{1}{f(x)})\).
  Let \(U = \theta(V_f)\), prove that \(T_p V \cong T_{\theta(p)} U\).
\end{problem}
\begin{solution}
  Write \(k[\mathbbm{A}_k^n]=k[x_1,\cdots , x_n ,y]\). Assume \(V = \van(I)= \van(f_1,\cdots, f_m)\), where \(f_i \in k[x_1,\cdots,x_n ]\).
  Then \(U = \van(f_1,\cdots,f_n, yf-1)\). Now consider \(\tau: T_p(V) \to \mathbbm{A}_k^{n+1}, \tau(x):=(x,\frac{1}{f(p)}-\frac{f_p^{(1)}(x)}{f^2(p)})\).
  Now we prove \(\tau(T_p V)=T_{\theta(p)} U\).
  Only need to prove \((yf-1)_{\theta(p)}^{(1)}(\tau(x))=0\).
  i.e., \(\frac{f_p^{(1)}(x)}{f(p)}+f(p)(y-\frac{1}{f(p)})=0\), where \(y = \frac{1}{f(p)}-\frac{f_p^{(1)}}{f^2(p)}\).
  Substitute \(y\) into the equation, we get is't obvious.

  Obviously \(\tau\) is injective, so it's isomorphic.
\end{solution}
\end{document}


